using standard op: insert

theory/x86CommType.thy
@@ -56,13 +56,19 @@ x86_sib_base  :: u8
 
 definition construct_rex_to_u8 :: "bool \<Rightarrow> bool \<Rightarrow> bool \<Rightarrow> bool \<Rightarrow> u8" where
 "construct_rex_to_u8 w r x b =
-  or (or (or  ((u8_of_bool w) << 3)
-              ((u8_of_bool r) << 2))
-          ((u8_of_bool x) << 1))
-     (u8_of_bool b)
+  bitfield_insert_u8 4 4
+    (bitfield_insert_u8 3 1
+      (bitfield_insert_u8 2 1
+        (bitfield_insert_u8 1 1 (u8_of_bool b)
+                                (u8_of_bool x))
+        (u8_of_bool r))
+    (u8_of_bool w)) 0x4
 "
 
 definition construct_modsib_to_u8 :: "u8 \<Rightarrow> u8 \<Rightarrow> u8 \<Rightarrow> u8" where
-"construct_modsib_to_u8 op1 op2 op3 = or (or ((and 0b11 op1) << 6) ((and 0b111 op2) << 3)) (and 0b111 op3)"
+"construct_modsib_to_u8 op1 op2 op3 =
+  bitfield_insert_u8 6 2
+    (bitfield_insert_u8 3 3 (and 0b111 op3) (and 0b111 op2))
+    0b11"
 
 end
