theory/x64Assembler.thy
@@ -14,7 +14,7 @@ fun x64_assemble_one_instruction :: "instruction \<Rightarrow> x64_bin option" w
   case ins of
   \<comment> \<open> P2882 `MOV register1 to register2` -> `0100 0R0B : 1000 1001 : 11 reg1 reg2` \<close>
   Pmovl_rr rd r1 \<Rightarrow>
-    let (rex:: u8) = or 0x40 (construct_rex_to_u8  \<comment> \<open> `0R0B` \<close>
+    let (rex:: u8) = (construct_rex_to_u8  \<comment> \<open> `0R0B` \<close>
       False \<comment> \<open> W \<close>
       (and (u8_of_ireg r1) 0b1000 \<noteq> 0) \<comment> \<open> R \<close>
       False \<comment> \<open> X \<close>
@@ -25,7 +25,7 @@ fun x64_assemble_one_instruction :: "instruction \<Rightarrow> x64_bin option" w
       Some [ rex, op, rop] |
   \<comment> \<open> P2882 `MOV qwordregister1 to qwordregister2` -> `0100 1R0B : 1000 1001 : 11 reg1 reg2` \<close>
   Pmovq_rr rd r1 \<Rightarrow>
-    let (rex:: u8) = or 0x40 (construct_rex_to_u8  \<comment> \<open> `1R0B` \<close>
+    let (rex:: u8) = (construct_rex_to_u8  \<comment> \<open> `1R0B` \<close>
       True \<comment> \<open> W \<close>
       (and (u8_of_ireg r1) 0b1000 \<noteq> 0) \<comment> \<open> R \<close>
       False \<comment> \<open> X \<close>
@@ -36,7 +36,7 @@ fun x64_assemble_one_instruction :: "instruction \<Rightarrow> x64_bin option" w
       Some [ rex, op, rop] |
   \<comment> \<open> P2876 `ADD register1 to register2` -> `0100 1R0B : 0000 000w : 11 reg1 reg2` \<close>
   Paddl_rr rd r1 \<Rightarrow>
-    let (rex:: u8) = or 0x40 (construct_rex_to_u8  \<comment> \<open> `0R0B` \<close>
+    let (rex:: u8) = (construct_rex_to_u8  \<comment> \<open> `0R0B` \<close>
       False \<comment> \<open> W \<close>
       (and (u8_of_ireg r1) 0b1000 \<noteq> 0) \<comment> \<open> R \<close>
       False \<comment> \<open> X \<close>
@@ -47,7 +47,7 @@ fun x64_assemble_one_instruction :: "instruction \<Rightarrow> x64_bin option" w
       Some [ rex, op, rop] |
   \<comment> \<open> P2876 `ADD qwordregister1 to qwordregister2` -> `0100 1R0B : 0000 0001 : 11 reg1 reg2` \<close>
   Paddq_rr rd r1 \<Rightarrow>
-    let (rex:: u8) = or 0x40 (construct_rex_to_u8  \<comment> \<open> `1R0B` \<close>
+    let (rex:: u8) = (construct_rex_to_u8  \<comment> \<open> `1R0B` \<close>
       True \<comment> \<open> W \<close>
       (and (u8_of_ireg r1) 0b1000 \<noteq> 0) \<comment> \<open> R \<close>
       False \<comment> \<open> X \<close>
@@ -58,7 +58,7 @@ fun x64_assemble_one_instruction :: "instruction \<Rightarrow> x64_bin option" w
       Some [ rex, op, rop] |
   \<comment> \<open> P2891 `SUB register1 from register2` -> `0100 0R0B : 0010 100w : 11 reg1 reg2` \<close>
   Psubl_rr rd r1 \<Rightarrow>
-    let (rex:: u8) = or 0x40 (construct_rex_to_u8  \<comment> \<open> `0R0B` \<close>
+    let (rex:: u8) = (construct_rex_to_u8  \<comment> \<open> `0R0B` \<close>
       False \<comment> \<open> W \<close>
       (and (u8_of_ireg r1) 0b1000 \<noteq> 0) \<comment> \<open> R \<close>
       False \<comment> \<open> X \<close>
@@ -69,7 +69,7 @@ fun x64_assemble_one_instruction :: "instruction \<Rightarrow> x64_bin option" w
       Some [ rex, op, rop] |
   \<comment> \<open> P2891 `SUB qwordregister1 from qwordregister2` -> `0100 1R0B : 0010 1001 : 11 reg1 reg2` \<close>
   Psubq_rr rd r1 \<Rightarrow>
-    let (rex:: u8) = or 0x40 (construct_rex_to_u8  \<comment> \<open> `1R0B` \<close>
+    let (rex:: u8) = (construct_rex_to_u8  \<comment> \<open> `1R0B` \<close>
       True \<comment> \<open> W \<close>
       (and (u8_of_ireg r1) 0b1000 \<noteq> 0) \<comment> \<open> R \<close>
       False \<comment> \<open> X \<close>
@@ -80,7 +80,7 @@ fun x64_assemble_one_instruction :: "instruction \<Rightarrow> x64_bin option" w
       Some [ rex, op, rop] |
   \<comment> \<open> P2884 `NEG register2` -> `0100 000B : 1111 011w : 11011reg` \<close>
   Pnegl rd \<Rightarrow>
-    let (rex:: u8) = or 0x40 (construct_rex_to_u8  \<comment> \<open> `000B` \<close>
+    let (rex:: u8) = (construct_rex_to_u8  \<comment> \<open> `000B` \<close>
       False \<comment> \<open> W \<close>
       False \<comment> \<open> R \<close>
       False \<comment> \<open> X \<close>
@@ -91,7 +91,7 @@ fun x64_assemble_one_instruction :: "instruction \<Rightarrow> x64_bin option" w
       Some [rex, op, rop] |
   \<comment> \<open> P2884 `NEG register2` -> `0100 100B : 1111 0111 : 11011reg` \<close>
   Pnegq rd \<Rightarrow>
-    let (rex:: u8) = or 0x40 (construct_rex_to_u8  \<comment> \<open> `100B` \<close>
+    let (rex:: u8) = (construct_rex_to_u8  \<comment> \<open> `100B` \<close>
       True \<comment> \<open> W \<close>
       False \<comment> \<open> R \<close>
       False \<comment> \<open> X \<close>
@@ -102,7 +102,7 @@ fun x64_assemble_one_instruction :: "instruction \<Rightarrow> x64_bin option" w
       Some [rex, op, rop] |
   \<comment> \<open> P2884 `OR register1 to register2` -> ` 0000 100w : 11 reg1 reg2` \<close>
   Porl_rr rd r1  \<Rightarrow> 
-     let (rex:: u8) = or 0x40 (construct_rex_to_u8  \<comment> \<open> `1R0B` \<close>
+     let (rex:: u8) = (construct_rex_to_u8  \<comment> \<open> `1R0B` \<close>
       False \<comment> \<open> W \<close>
       (and (u8_of_ireg r1) 0b1000 \<noteq> 0) \<comment> \<open> R \<close>
       False \<comment> \<open> X \<close>
@@ -113,7 +113,7 @@ fun x64_assemble_one_instruction :: "instruction \<Rightarrow> x64_bin option" w
       Some [ rex, op, rop] |
   \<comment> \<open> P2884 `OR qwordregister1 to qwordregister2` -> ` 0100 1R0B : 0000 1001 : 11 reg1 reg2` \<close>
   Porq_rr rd r1  \<Rightarrow> 
-     let (rex:: u8) = or 0x40 (construct_rex_to_u8  \<comment> \<open> `1R0B` \<close>
+     let (rex:: u8) = (construct_rex_to_u8  \<comment> \<open> `1R0B` \<close>
       True \<comment> \<open> W \<close>
       (and (u8_of_ireg r1) 0b1000 \<noteq> 0) \<comment> \<open> R \<close>
       False \<comment> \<open> X \<close>
@@ -124,7 +124,7 @@ fun x64_assemble_one_instruction :: "instruction \<Rightarrow> x64_bin option" w
       Some [ rex, op, rop] |
   \<comment> \<open> P2876 `AND register1 to register2` -> ` 0100 0R0B : 0010 000w : 11 reg1 reg2` \<close>
   Pandl_rr rd r1  \<Rightarrow> 
-     let (rex:: u8) = or 0x40 (construct_rex_to_u8  \<comment> \<open> `0R0B` \<close>
+     let (rex:: u8) = (construct_rex_to_u8  \<comment> \<open> `0R0B` \<close>
       False \<comment> \<open> W \<close>
       (and (u8_of_ireg r1) 0b1000 \<noteq> 0) \<comment> \<open> R \<close>
       False \<comment> \<open> X \<close>
@@ -135,7 +135,7 @@ fun x64_assemble_one_instruction :: "instruction \<Rightarrow> x64_bin option" w
       Some [ rex, op, rop] |
   \<comment> \<open> P2876 `AND qwordregister1 to qwordregister2` -> ` 0100 1R0B : 0010 0001 : 11 reg1 reg2` \<close>
   Pandq_rr rd r1  \<Rightarrow> 
-     let (rex:: u8) = or 0x40 (construct_rex_to_u8  \<comment> \<open> `1R0B` \<close>
+     let (rex:: u8) = (construct_rex_to_u8  \<comment> \<open> `1R0B` \<close>
       True \<comment> \<open> W \<close>
       (and (u8_of_ireg r1) 0b1000 \<noteq> 0) \<comment> \<open> R \<close>
       False \<comment> \<open> X \<close>
@@ -146,7 +146,7 @@ fun x64_assemble_one_instruction :: "instruction \<Rightarrow> x64_bin option" w
       Some [ rex, op, rop] |
   \<comment> \<open> P2893 `XOR register1 to register2` -> ` 0100 0RXB : 0011 000w : 11 reg1 reg2` \<close>
   Pxorl_rr rd r1  \<Rightarrow> 
-     let (rex:: u8) = or 0x40 (construct_rex_to_u8  \<comment> \<open> `0R0B` \<close>
+     let (rex:: u8) = (construct_rex_to_u8  \<comment> \<open> `0R0B` \<close>
       False \<comment> \<open> W \<close>
       (and (u8_of_ireg r1) 0b1000 \<noteq> 0) \<comment> \<open> R \<close>
       False \<comment> \<open> X \<close>
@@ -157,7 +157,7 @@ fun x64_assemble_one_instruction :: "instruction \<Rightarrow> x64_bin option" w
       Some [ rex, op, rop] |
   \<comment> \<open> P2893 `XOR qwordregister1 to qwordregister2` -> ` 0100 1R0B : 0011 0001 : 11 reg1 reg2` \<close>
   Pxorq_rr rd r1  \<Rightarrow> 
-     let (rex:: u8) = or 0x40 (construct_rex_to_u8  \<comment> \<open> `1R0B` \<close>
+     let (rex:: u8) = (construct_rex_to_u8  \<comment> \<open> `1R0B` \<close>
       True \<comment> \<open> W \<close>
       (and (u8_of_ireg r1) 0b1000 \<noteq> 0) \<comment> \<open> R \<close>
       False \<comment> \<open> X \<close>
@@ -168,7 +168,7 @@ fun x64_assemble_one_instruction :: "instruction \<Rightarrow> x64_bin option" w
       Some [ rex, op, rop] |
   \<comment> \<open> P2884 `MUL AL, AX, or EAX with register2` -> ` 0100 000B : 1111 011w : 11 100 reg` \<close>
   Pmull_r r1 \<Rightarrow>
-    let (rex:: u8) = or 0x40 (construct_rex_to_u8  \<comment> \<open> `000B` \<close>
+    let (rex:: u8) = (construct_rex_to_u8  \<comment> \<open> `000B` \<close>
       False \<comment> \<open> W \<close>
       False \<comment> \<open> R \<close>
       False \<comment> \<open> X \<close>
@@ -179,7 +179,7 @@ fun x64_assemble_one_instruction :: "instruction \<Rightarrow> x64_bin option" w
       Some [ rex, op, rop] |
   \<comment> \<open> P2884 `MUL RAX with qwordregister (to RDX:RAX)` -> ` 0100 100B : 1111 0111 : 11 100 qowrdreg` \<close>
   Pmulq_r r1 \<Rightarrow>
-    let (rex:: u8) = or 0x40 (construct_rex_to_u8  \<comment> \<open> `100B` \<close>
+    let (rex:: u8) = (construct_rex_to_u8  \<comment> \<open> `100B` \<close>
       True \<comment> \<open> W \<close>
       False \<comment> \<open> R \<close>
       False \<comment> \<open> X \<close>
@@ -190,7 +190,7 @@ fun x64_assemble_one_instruction :: "instruction \<Rightarrow> x64_bin option" w
       Some [ rex, op, rop] |
   \<comment> \<open> P2880 `IMUL AL, AX, or EAX with register2` -> ` 0100 000B : 1111 011w : 11 101 reg` \<close>
   Pimull_r r1 \<Rightarrow>
-    let (rex:: u8) = or 0x40 (construct_rex_to_u8  \<comment> \<open> `000B` \<close>
+    let (rex:: u8) = (construct_rex_to_u8  \<comment> \<open> `000B` \<close>
       False \<comment> \<open> W \<close>
       False \<comment> \<open> R \<close>
       False \<comment> \<open> X \<close>
@@ -201,7 +201,7 @@ fun x64_assemble_one_instruction :: "instruction \<Rightarrow> x64_bin option" w
       Some [ rex, op, rop] |
   \<comment> \<open> P2880 `IMUL RAX with qwordregister (to RDX:RAX)` -> ` 0100 100B : 1111 0111 : 11 101 qwordreg` \<close>
   Pimulq_r r1 \<Rightarrow>
-    let (rex:: u8) = or 0x40 (construct_rex_to_u8  \<comment> \<open> `100B` \<close>
+    let (rex:: u8) = (construct_rex_to_u8  \<comment> \<open> `100B` \<close>
       True \<comment> \<open> W \<close>
       False \<comment> \<open> R \<close>
       False \<comment> \<open> X \<close>
@@ -212,7 +212,7 @@ fun x64_assemble_one_instruction :: "instruction \<Rightarrow> x64_bin option" w
       Some [ rex, op, rop] |
   \<comment> \<open> P2879 `DIV AL, AX, or EAX by register2` -> ` 0100 000B : 1111 011w : 11 110eg` \<close>
   Pdivl_r r1 \<Rightarrow>
-    let (rex:: u8) = or 0x40 (construct_rex_to_u8  \<comment> \<open> `000B` \<close>
+    let (rex:: u8) = (construct_rex_to_u8  \<comment> \<open> `000B` \<close>
       False \<comment> \<open> W \<close>
       False \<comment> \<open> R \<close>
       False \<comment> \<open> X \<close>
@@ -223,7 +223,7 @@ fun x64_assemble_one_instruction :: "instruction \<Rightarrow> x64_bin option" w
       Some [ rex, op, rop] |
   \<comment> \<open> P2879 `DIV EAX by qwordregister (to RDX:RAX)` -> ` 0100 100B : 1111 0111 : 11 110 qwordreg` \<close>
   Pdivq_r r1 \<Rightarrow>
-    let (rex:: u8) = or 0x40 (construct_rex_to_u8  \<comment> \<open> `100B` \<close>
+    let (rex:: u8) = (construct_rex_to_u8  \<comment> \<open> `100B` \<close>
       True \<comment> \<open> W \<close>
       False \<comment> \<open> R \<close>
       False \<comment> \<open> X \<close>
@@ -234,7 +234,7 @@ fun x64_assemble_one_instruction :: "instruction \<Rightarrow> x64_bin option" w
       Some [ rex, op, rop] |
   \<comment> \<open> P2879 `IDIV AL, AX, or EAX by register2` -> ` 0100 000B : 1111 011w : 11 111 reg` \<close>
   Pidivl_r r1 \<Rightarrow>
-    let (rex:: u8) = or 0x40 (construct_rex_to_u8  \<comment> \<open> `000B` \<close>
+    let (rex:: u8) = (construct_rex_to_u8  \<comment> \<open> `000B` \<close>
       False \<comment> \<open> W \<close>
       False \<comment> \<open> R \<close>
       False \<comment> \<open> X \<close>
@@ -245,7 +245,7 @@ fun x64_assemble_one_instruction :: "instruction \<Rightarrow> x64_bin option" w
       Some [ rex, op, rop] |
   \<comment> \<open> P2879 `IDIV RAX by qwordregister (to RDX:RAX)` -> ` 0100 100B : 1111 0111 : 11 111 qwordreg` \<close>
   Pidivq_r r1 \<Rightarrow>
-    let (rex:: u8) = or 0x40 (construct_rex_to_u8  \<comment> \<open> `100B` \<close>
+    let (rex:: u8) = (construct_rex_to_u8  \<comment> \<open> `100B` \<close>
       True \<comment> \<open> W \<close>
       False \<comment> \<open> R \<close>
       False \<comment> \<open> X \<close>
@@ -256,7 +256,7 @@ fun x64_assemble_one_instruction :: "instruction \<Rightarrow> x64_bin option" w
       Some [ rex, op, rop] |
   \<comment> \<open> P2889 `SHL register by immediate count`      -> ` 0100 000B 1100 000w : 11 100 reg : imm8 ` \<close>
   Pshll_ri rd n \<Rightarrow>
-    let (rex:: u8) = or 0x40 (construct_rex_to_u8  \<comment> \<open> `000B` \<close>
+    let (rex:: u8) = (construct_rex_to_u8  \<comment> \<open> `000B` \<close>
       False \<comment> \<open> W \<close>
       False \<comment> \<open> R \<close>
       False \<comment> \<open> X \<close>
@@ -268,7 +268,7 @@ fun x64_assemble_one_instruction :: "instruction \<Rightarrow> x64_bin option" w
       Some [ rex, op, rop, imm] |
   \<comment> \<open> P2889 `SHL qwordregister by immediate count` -> ` 0100 100B 1100 0001 : 11 100 reg : imm8 ` \<close>
   Pshlq_ri rd n \<Rightarrow>
-    let (rex:: u8) = or 0x40 (construct_rex_to_u8  \<comment> \<open> `100B` \<close>
+    let (rex:: u8) = (construct_rex_to_u8  \<comment> \<open> `100B` \<close>
       True \<comment> \<open> W \<close>
       False \<comment> \<open> R \<close>
       False \<comment> \<open> X \<close>
@@ -280,7 +280,7 @@ fun x64_assemble_one_instruction :: "instruction \<Rightarrow> x64_bin option" w
       Some [ rex, op, rop, imm] |
   \<comment> \<open> P2889 `SHL register by CL`                   -> ` 0100 000B 1101 001w : 11 100 reg ` \<close>
   Pshll_r rd  \<Rightarrow>
-    let (rex:: u8) = or 0x40 (construct_rex_to_u8  \<comment> \<open> `000B` \<close>
+    let (rex:: u8) = (construct_rex_to_u8  \<comment> \<open> `000B` \<close>
       False \<comment> \<open> W \<close>
       False \<comment> \<open> R \<close>
       False \<comment> \<open> X \<close>
@@ -291,7 +291,7 @@ fun x64_assemble_one_instruction :: "instruction \<Rightarrow> x64_bin option" w
       Some [ rex, op, rop] |
   \<comment> \<open> P2889 `SHL qwordregister by CL`              -> ` 0100 100B 1101 001w : 11 100 reg ` \<close>
   Pshlq_r rd  \<Rightarrow>
-    let (rex:: u8) = or 0x40 (construct_rex_to_u8  \<comment> \<open> `100B` \<close>
+    let (rex:: u8) = (construct_rex_to_u8  \<comment> \<open> `100B` \<close>
       True \<comment> \<open> W \<close>
       False \<comment> \<open> R \<close>
       False \<comment> \<open> X \<close>
@@ -302,7 +302,7 @@ fun x64_assemble_one_instruction :: "instruction \<Rightarrow> x64_bin option" w
       Some [ rex, op, rop ] |
   \<comment> \<open> P2890 `SHR register by immediate count`      -> ` 0100 000B 1100 000w : 11 101 reg : imm8 ` \<close>
   Pshrl_ri rd n \<Rightarrow>
-    let (rex:: u8) = or 0x40 (construct_rex_to_u8  \<comment> \<open> `000B` \<close>
+    let (rex:: u8) = (construct_rex_to_u8  \<comment> \<open> `000B` \<close>
       False \<comment> \<open> W \<close>
       False \<comment> \<open> R \<close>
       False \<comment> \<open> X \<close>
@@ -314,7 +314,7 @@ fun x64_assemble_one_instruction :: "instruction \<Rightarrow> x64_bin option" w
       Some [ rex, op, rop, imm] |
   \<comment> \<open> P2890 `SHR qwordregister by immediate count` -> ` 0100 100B 1100 000w : 11 101 reg : imm8 ` \<close>
   Pshrq_ri rd n \<Rightarrow>
-    let (rex:: u8) = or 0x40 (construct_rex_to_u8  \<comment> \<open> `100B` \<close>
+    let (rex:: u8) = (construct_rex_to_u8  \<comment> \<open> `100B` \<close>
       True \<comment> \<open> W \<close>
       False \<comment> \<open> R \<close>
       False \<comment> \<open> X \<close>
@@ -326,7 +326,7 @@ fun x64_assemble_one_instruction :: "instruction \<Rightarrow> x64_bin option" w
       Some [ rex, op, rop, imm] |
   \<comment> \<open> P2890 `SHR register by CL`                   -> ` 0100 000B 1101 001w : 11 101 reg ` \<close>
   Pshrl_r rd  \<Rightarrow>
-    let (rex:: u8) = or 0x40 (construct_rex_to_u8  \<comment> \<open> `000B` \<close>
+    let (rex:: u8) = (construct_rex_to_u8  \<comment> \<open> `000B` \<close>
       False \<comment> \<open> W \<close>
       False \<comment> \<open> R \<close>
       False \<comment> \<open> X \<close>
@@ -337,7 +337,7 @@ fun x64_assemble_one_instruction :: "instruction \<Rightarrow> x64_bin option" w
       Some [ rex, op, rop ] |
   \<comment> \<open> P2890 `SHR qwrodregister by CL`              -> ` 0100 100B 1101 001w : 11 101 reg ` \<close>
   Pshrq_r rd  \<Rightarrow>
-    let (rex:: u8) = or 0x40 (construct_rex_to_u8  \<comment> \<open> `100B` \<close>
+    let (rex:: u8) = (construct_rex_to_u8  \<comment> \<open> `100B` \<close>
       True \<comment> \<open> W \<close>
       False \<comment> \<open> R \<close>
       False \<comment> \<open> X \<close>
@@ -348,7 +348,7 @@ fun x64_assemble_one_instruction :: "instruction \<Rightarrow> x64_bin option" w
       Some [ rex, op, rop ] |
   \<comment> \<open> P2888 `SAR register by immediate count`      -> ` 0100 000B 1100 000w : 11 111 reg : imm8 ` \<close>
   Psarl_ri rd n \<Rightarrow>
-    let (rex:: u8) = or 0x40 (construct_rex_to_u8  \<comment> \<open> `000B` \<close>
+    let (rex:: u8) = (construct_rex_to_u8  \<comment> \<open> `000B` \<close>
       False \<comment> \<open> W \<close>
       False \<comment> \<open> R \<close>
       False \<comment> \<open> X \<close>
@@ -360,7 +360,7 @@ fun x64_assemble_one_instruction :: "instruction \<Rightarrow> x64_bin option" w
       Some [ rex, op, rop, imm] |
   \<comment> \<open> P2888 `SAR qwordregister by immediate count` -> ` 0100 100B 1100 000w : 11 111 reg : imm8 ` \<close>
   Psarq_ri rd n \<Rightarrow>
-    let (rex:: u8) = or 0x40 (construct_rex_to_u8  \<comment> \<open> `100B` \<close>
+    let (rex:: u8) = (construct_rex_to_u8  \<comment> \<open> `100B` \<close>
       True \<comment> \<open> W \<close>
       False \<comment> \<open> R \<close>
       False \<comment> \<open> X \<close>
@@ -372,7 +372,7 @@ fun x64_assemble_one_instruction :: "instruction \<Rightarrow> x64_bin option" w
       Some [ rex, op, rop, imm] |
   \<comment> \<open> P2888 `SAR register by CL`                   -> ` 0100 000B 1101 001w : 11 111 reg ` \<close>
   Psarl_r rd  \<Rightarrow>
-    let (rex:: u8) = or 0x40 (construct_rex_to_u8  \<comment> \<open> `000B` \<close>
+    let (rex:: u8) = (construct_rex_to_u8  \<comment> \<open> `000B` \<close>
       False \<comment> \<open> W \<close>
       False \<comment> \<open> R \<close>
       False \<comment> \<open> X \<close>
@@ -383,7 +383,7 @@ fun x64_assemble_one_instruction :: "instruction \<Rightarrow> x64_bin option" w
       Some [ rex, op, rop ] |
   \<comment> \<open> P2888 `SAR qwordregister by CL`              -> ` 0100 100B 1101 001w : 11 111 reg ` \<close>
   Psarq_r rd  \<Rightarrow>
-    let (rex:: u8) = or 0x40 (construct_rex_to_u8  \<comment> \<open> `100B` \<close>
+    let (rex:: u8) = (construct_rex_to_u8  \<comment> \<open> `100B` \<close>
       True \<comment> \<open> W \<close>
       False \<comment> \<open> R \<close>
       False \<comment> \<open> X \<close>
