theory/x64ConsistencyProof2Pmov0.thy
@@ -11,13 +11,11 @@ lemma [simp]: "((and (and 7 d) (- 9))) = ((and 7 d)::u8)"
     apply (auto simp add: bit_simps)
     apply (simp add: bit_iff_odd)
     apply (cases n, simp_all)
-    subgoal for n1
-      apply (cases n1, simp_all)
-    subgoal for n2
-      apply (cases n2, simp_all)
+    subgoal for n1 apply (cases n1, simp_all)
+      subgoal for n2 apply (cases n2, simp_all)
+        done
       done
     done
-  done
   done
 
 lemma [simp]: "and 15 ((rex::u8) >> 4) = 4 \<Longrightarrow>
@@ -31,23 +29,17 @@ bit rex (Suc (Suc (Suc (Suc (Suc (Suc 0))))))"
 
 lemma mov_subgoal1: "and 15 (rex >> 4) = (4::u8) \<Longrightarrow> n < 8 \<Longrightarrow> bit 64 n \<Longrightarrow> bit rex n"
   apply (cases n, simp_all)
-  subgoal for n1
-    apply (cases n1, simp_all)
+  subgoal for n1 apply (cases n1, simp_all)
     subgoal by (simp add: bit_numeral_Bit0_iff)
-    subgoal for n2
-      apply (cases n2, simp_all)
+    subgoal for n2 apply (cases n2, simp_all)
       subgoal by (simp add: bit_numeral_Bit0_iff)
-      subgoal for n3
-        apply (cases n3, simp_all)
+      subgoal for n3 apply (cases n3, simp_all)
         subgoal by (simp add: bit_numeral_Bit0_iff)
-        subgoal for n4
-          apply (cases n4, simp_all)
+        subgoal for n4 apply (cases n4, simp_all)
           subgoal by (simp add: bit_numeral_Bit0_iff)
-          subgoal for n5
-            apply (cases n5, simp_all)
+          subgoal for n5 apply (cases n5, simp_all)
             subgoal by (simp add: bit_numeral_Bit0_iff)
-            subgoal for n6
-              apply (cases n6, simp_all)
+            subgoal for n6 apply (cases n6, simp_all)
               subgoal for n7
                 by (metis bit_double_Suc_iff bit_exp_iff mult_1_right not_bit_numeral_Bit0_0 numeral_Bit0_eq_double power.simps(1))
               done
@@ -58,23 +50,20 @@ lemma mov_subgoal1: "and 15 (rex >> 4) = (4::u8) \<Longrightarrow> n < 8 \<Longr
     done
   done
 
-lemma [simp]: "and 1 (rex >> 3) = 1 \<Longrightarrow> bit rex (Suc (Suc (Suc 0)))"
+lemma [simp]: "and 1 ((rex::u8) >> 3) = 1 \<Longrightarrow> bit rex (Suc (Suc (Suc 0)))"
   apply (simp add: bit_eq_iff)
   apply (auto simp add: bit_simps)
   apply (drule_tac x="0" in spec)
   apply (simp add: eval_nat_numeral(2) eval_nat_numeral(3))
   done
 
-lemma mov_subgoal2: "and 1 (rex >> 3) = 1 \<Longrightarrow> n < 8 \<Longrightarrow> bit 8 n \<Longrightarrow> bit rex n"
+lemma mov_subgoal2: "and 1 ((rex::u8) >> 3) = 1 \<Longrightarrow> n < 8 \<Longrightarrow> bit 8 n \<Longrightarrow> bit rex n"
   apply (cases n, simp_all)
-  subgoal for n1
-    apply (cases n1, simp_all)
+  subgoal for n1 apply (cases n1, simp_all)
     subgoal by (simp add: bit_numeral_Bit0_iff)
-    subgoal for n2
-      apply (cases n2, simp_all)
+    subgoal for n2 apply (cases n2, simp_all)
       subgoal by (simp add: bit_numeral_Bit0_iff)
-      subgoal for n3
-        apply (cases n3, simp_all)
+      subgoal for n3 apply (cases n3, simp_all)
         subgoal for n4
           by (simp add: bit_1_iff bit_numeral_Bit0_iff)
         done
@@ -82,7 +71,7 @@ lemma mov_subgoal2: "and 1 (rex >> 3) = 1 \<Longrightarrow> n < 8 \<Longrightarr
     done
   done
 
-lemma mov_subgoal3_1: "and (or (and 8 ((rex >> 2) << 3)) (and (7::u8) (rop >> 3))) 8 \<noteq> 0 \<Longrightarrow>
+lemma mov_subgoal3_1: "and (or (and 8 (((rex::u8) >> 2) << 3)) (and (7::u8) (rop >> 3))) 8 \<noteq> 0 \<Longrightarrow>
     bit rex (Suc (Suc 0))"
   apply (erule contrapos_pp)
   apply simp
@@ -94,10 +83,8 @@ lemma mov_subgoal3_1: "and (or (and 8 ((rex >> 2) << 3)) (and (7::u8) (rop >> 3)
       by (metis One_nat_def Suc_diff_diff bit_2_iff bit_numeral_Bit0_iff diff_zero numeral_3_eq_3)
     subgoal 
       apply (cases n, simp_all)
-      subgoal for n1
-        apply (cases n1, simp_all)
-        subgoal for n2
-          apply (cases n2, simp_all)
+      subgoal for n1 apply (cases n1, simp_all)
+        subgoal for n2 apply (cases n2, simp_all)
           done
         done
       done
@@ -114,24 +101,17 @@ lemma mov_subgoal3: "and 15 ((rex::u8) >> 4) = 4 \<Longrightarrow>
     bit rex n"
   apply (cases "and (or (and 8 ((rex >> 2) << 3)) (and 7 (rop >> 3))) 8 \<noteq> 0", simp_all)
   apply (cases n, simp_all)
-  subgoal for n1
-    apply (cases n1, simp_all)
-    subgoal for n2
-      apply (cases n2, simp_all)
+  subgoal for n1 apply (cases n1, simp_all)
+    subgoal for n2 apply (cases n2, simp_all)
       subgoal using mov_subgoal3_1 by blast
-      subgoal for n3
-      apply (cases n3, simp_all)
-        subgoal for n4
-          apply (cases n4, simp_all)
+      subgoal for n3 apply (cases n3, simp_all)
+        subgoal for n4 apply (cases n4, simp_all)
           subgoal using bit_1_iff by blast
-          subgoal for n5
-            apply (cases n5, simp_all)
+          subgoal for n5 apply (cases n5, simp_all)
             subgoal using bit_1_iff by blast
-            subgoal for n6
-              apply (cases n6, simp_all)
+            subgoal for n6 apply (cases n6, simp_all)
               subgoal using bit_1_iff by blast
-              subgoal for n7
-                apply (cases n7, simp_all)
+              subgoal for n7 apply (cases n7, simp_all)
                 subgoal using bit_1_iff by blast
                 done
               done
@@ -142,7 +122,7 @@ lemma mov_subgoal3: "and 15 ((rex::u8) >> 4) = 4 \<Longrightarrow>
     done
   done
 
-lemma [simp]: "and (or (and 8 (rex << 3)) (and 7 rop)) 8 \<noteq> 0 \<Longrightarrow> bit rex 0"
+lemma [simp]: "and (or (and 8 ((rex::u8) << 3)) (and 7 rop)) 8 \<noteq> 0 \<Longrightarrow> bit rex 0"
   apply (erule contrapos_pp)
   apply simp
   apply (rule bit_eqI)
@@ -153,17 +133,15 @@ lemma [simp]: "and (or (and 8 (rex << 3)) (and 7 rop)) 8 \<noteq> 0 \<Longrighta
       by (metis One_nat_def Suc_diff_diff bit_2_iff bit_numeral_Bit0_iff diff_zero numeral_3_eq_3)
     subgoal 
       apply (cases n, simp_all)
-      subgoal for n1
-        apply (cases n1, simp_all)
-        subgoal for n2
-          apply (cases n2, simp_all)
+      subgoal for n1 apply (cases n1, simp_all)
+        subgoal for n2 apply (cases n2, simp_all)
           done
         done
       done
     done
   done
 
-lemma mov_subgoal4: "and 15 (rex >> 4) = 4 \<Longrightarrow>
+lemma mov_subgoal4: "and 15 ((rex::u8) >> 4) = 4 \<Longrightarrow>
     and 1 (rex >> 3) = 1 \<Longrightarrow>
     and 1 (rex >> Suc 0) = 0 \<Longrightarrow>
     n < 8 \<Longrightarrow>
@@ -171,25 +149,18 @@ lemma mov_subgoal4: "and 15 (rex >> 4) = 4 \<Longrightarrow>
     bit rex n"
   apply (cases "and (or (and 8 (rex << 3)) (and 7 rop)) 8 \<noteq> 0", simp_all)
   apply (cases n, simp_all)
-  subgoal for n1
-    apply (cases n1, simp_all)
+  subgoal for n1 apply (cases n1, simp_all)
     subgoal using bit_1_iff by blast
-    subgoal for n2
-      apply (cases n2, simp_all)
+    subgoal for n2 apply (cases n2, simp_all)
       subgoal using bit_1_iff by blast
-      subgoal for n3
-      apply (cases n3, simp_all)
-        subgoal for n4
-          apply (cases n4, simp_all)
+      subgoal for n3 apply (cases n3, simp_all)
+        subgoal for n4 apply (cases n4, simp_all)
           subgoal using bit_1_iff by blast
-          subgoal for n5
-            apply (cases n5, simp_all)
+          subgoal for n5 apply (cases n5, simp_all)
             subgoal using bit_1_iff by blast
-            subgoal for n6
-              apply (cases n6, simp_all)
+            subgoal for n6 apply (cases n6, simp_all)
               subgoal using bit_1_iff by blast
-              subgoal for n7
-                apply (cases n7, simp_all)
+              subgoal for n7 apply (cases n7, simp_all)
                 subgoal using bit_1_iff by blast
                 done
               done
@@ -200,19 +171,104 @@ lemma mov_subgoal4: "and 15 (rex >> 4) = 4 \<Longrightarrow>
     done
   done
 
-lemma mov_subgoal5_1: "bit rex 0 \<Longrightarrow> and (or (and 8 (rex << 3)) (and 7 rop)) (8::u8) = 0 \<Longrightarrow> False"
+lemma mov_subgoal5_1 [simp]: "and 15 ((rex::u8) >> 4) = 4 \<Longrightarrow>
+    bit rex (Suc (Suc (Suc (Suc 0)))) \<Longrightarrow> False"
+  by (metis bit_1_0 bit_and_iff bit_iff_and_drop_bit_eq_1 bit_numeral_Bit1_0 eval_nat_numeral(2) not_bit_numeral_Bit0_0 numeral_3_eq_3 semiring_norm(26) semiring_norm(27)) 
+          
+lemma mov_subgoal5_2 [simp]: "and 15 ((rex::u8) >> 4) = 4 \<Longrightarrow>
+    bit rex (Suc (Suc (Suc (Suc (Suc 0))))) \<Longrightarrow> False"
+  apply (simp add: bit_eq_iff)
+  apply (auto simp add: bit_simps)
+  apply (drule_tac x="1" in spec)
+  apply (simp add: eval_nat_numeral(2) eval_nat_numeral(3))
+  done
+
+lemma mov_subgoal5_3 [simp]: "and 15 ((rex::u8) >> 4) = 4 \<Longrightarrow>
+    bit rex (Suc (Suc (Suc (Suc (Suc (Suc (Suc 0))))))) \<Longrightarrow> False"
   apply (simp add: bit_eq_iff)
   apply (auto simp add: bit_simps)
   apply (drule_tac x="3" in spec)
   apply (simp add: eval_nat_numeral(2) eval_nat_numeral(3))
   done
 
-lemma mov_subgoal5_2: "and 1 (rex >> Suc 0) = 0 \<Longrightarrow> bit rex (Suc 0) \<Longrightarrow> False"
+lemma mov_subgoal5_4 [simp]: "bit (rex::u8) 0 \<Longrightarrow>
+    and (or (and 8 (rex << 3)) (and 7 rop)) 8 = 0 \<Longrightarrow> False"
+  apply (simp add: bit_eq_iff)
+  apply (auto simp add: bit_simps)
+  apply (drule_tac x="3" in spec)
+  apply (simp add: eval_nat_numeral(2) eval_nat_numeral(3))
+  done
+
+lemma mov_subgoal5: "and 15 ((rex::u8) >> 4) = 4 \<Longrightarrow>
+    and 1 (rex >> 3) = 1 \<Longrightarrow>
+    and 1 (rex >> Suc 0) = 0 \<Longrightarrow>
+    n < 8 \<Longrightarrow> bit rex n \<Longrightarrow>
+    \<not> bit (64::int) n \<Longrightarrow>
+    \<not> bit (8::int) n \<Longrightarrow>
+    \<not> bit (case and (or (and 8 (rex << 3)) (and 7 rop)) 8 \<noteq> 0 of True \<Rightarrow> 1 | False \<Rightarrow> 0)
+        n \<Longrightarrow>
+    bit (4::int) n"
+  apply (cases "and (or (and 8 (rex << 3)) (and 7 rop)) 8 \<noteq> 0", simp_all)
+  subgoal
+    apply (cases n, simp_all)
+    subgoal using bit_1_iff by blast
+    subgoal for n1 apply (cases n1, simp_all)
+      subgoal by (simp add: bit_word_iff_drop_bit_and word_bw_comms(1))
+      subgoal for n2 apply (cases n2, simp_all)
+      subgoal for n3 apply (cases n3, simp_all)
+        subgoal for n4 apply (cases n4, simp_all)
+          subgoal using mov_subgoal5_1 by blast
+          subgoal for n5 apply (cases n5, simp_all)
+            subgoal using mov_subgoal5_2 by blast
+            subgoal for n6 apply (cases n6, simp_all)
+              subgoal for n7 apply (cases n7, simp_all)
+                subgoal using mov_subgoal5_3 by blast
+                done
+              done
+            done
+          done
+        done
+      done
+    done
+  done
+  subgoal
+    apply (cases n, simp_all)
+    subgoal using mov_subgoal5_4 by blast
+    subgoal for n1 apply (cases n1, simp_all)
+      subgoal by (simp add: bit_word_iff_drop_bit_and word_bw_comms(1))
+      subgoal for n2 apply (cases n2, simp_all)
+        subgoal for n3 apply (cases n3, simp_all)
+          subgoal for n4 apply (cases n4, simp_all)
+            subgoal using mov_subgoal5_1 by blast
+            subgoal for n5 apply (cases n5, simp_all)
+              subgoal using mov_subgoal5_2 by blast
+              subgoal for n6 apply (cases n6, simp_all)
+                subgoal for n7 apply (cases n7, simp_all)
+                  subgoal using mov_subgoal5_3 by blast
+                  done
+                done
+              done
+            done
+          done
+        done
+      done
+    done
+  done
+
+
+lemma mov_subgoal6_1: "bit rex 0 \<Longrightarrow> and (or (and 8 (rex << 3)) (and 7 rop)) (8::u8) = 0 \<Longrightarrow> False"
+  apply (simp add: bit_eq_iff)
+  apply (auto simp add: bit_simps)
+  apply (drule_tac x="3" in spec)
+  apply (simp add: eval_nat_numeral(2) eval_nat_numeral(3))
+  done
+
+lemma mov_subgoal6_2: "and 1 (rex >> Suc 0) = 0 \<Longrightarrow> bit rex (Suc 0) \<Longrightarrow> False"
   apply (simp add: bit_eq_iff)
   apply (auto simp add: bit_simps)
   done
 
-lemma mov_subgoal5: "and 15 ((rex::u8) >> 4) = 4 \<Longrightarrow>
+lemma mov_subgoal6: "and 15 ((rex::u8) >> 4) = 4 \<Longrightarrow>
     and 1 (rex >> 3) = 1 \<Longrightarrow>
     and 1 (rex >> Suc 0) = 0 \<Longrightarrow>
     n < 8 \<Longrightarrow>
@@ -233,17 +289,18 @@ lemma mov_subgoal5: "and 15 ((rex::u8) >> 4) = 4 \<Longrightarrow>
     done
   subgoal
     apply (cases n, simp_all)
-    subgoal using mov_subgoal5_1 by blast
+    subgoal using mov_subgoal6_1 by blast
     subgoal for n1
       apply (cases n1, simp_all)
-      subgoal using mov_subgoal5_2 by blast
+      subgoal using mov_subgoal6_2 by blast
       done
     done
   done
 
 lemma [simp]: "\<not> bit (8::int) (Suc (Suc (Suc 0))) = False" by simp  
 
-lemma mov_subgoal6_1: "and 15 ((rex::u8) >> 4) = 4 \<Longrightarrow>
+(*
+lemma mov_subgoal12_1: "and 15 ((rex::u8) >> 4) = 4 \<Longrightarrow>
     bit rex (Suc (Suc (Suc (Suc 0)))) \<Longrightarrow> False"
   apply (simp add: bit_eq_iff)
   apply (auto simp add: bit_simps)
@@ -251,7 +308,7 @@ lemma mov_subgoal6_1: "and 15 ((rex::u8) >> 4) = 4 \<Longrightarrow>
   apply (simp add: eval_nat_numeral(2) eval_nat_numeral(3))
   done
 
-lemma mov_subgoal6_2: "and 15 (rex >> 4) = (4::u8) \<Longrightarrow>
+lemma mov_subgoal12_2: "and 15 (rex >> 4) = (4::u8) \<Longrightarrow>
     bit rex (Suc (Suc (Suc (Suc (Suc 0))))) \<Longrightarrow> False"
   apply (simp add: bit_eq_iff)
   apply (auto simp add: bit_simps)
@@ -261,7 +318,7 @@ lemma mov_subgoal6_2: "and 15 (rex >> 4) = (4::u8) \<Longrightarrow>
 
 lemma [simp]: "\<not> bit (64::int) (Suc (Suc (Suc (Suc (Suc (Suc 0)))))) \<Longrightarrow> False" by simp
 
-lemma mov_subgoal6_3: "and 15 (rex >> 4) = (4::u8) \<Longrightarrow>
+lemma mov_subgoal12_3: "and 15 (rex >> 4) = (4::u8) \<Longrightarrow>
     bit rex (Suc (Suc (Suc (Suc (Suc (Suc (Suc 0))))))) \<Longrightarrow> False"
   apply (simp add: bit_eq_iff)
   apply (auto simp add: bit_simps)
@@ -269,7 +326,7 @@ lemma mov_subgoal6_3: "and 15 (rex >> 4) = (4::u8) \<Longrightarrow>
   apply (simp add: eval_nat_numeral(2) eval_nat_numeral(3))
   done
 
-lemma mov_subgoal6_4: "and 1 (rex >> Suc 0) = (0::u8) \<Longrightarrow>
+lemma mov_subgoal12_4: "and 1 (rex >> Suc 0) = (0::u8) \<Longrightarrow>
     bit rex (Suc 0) \<Longrightarrow> False"
   apply (simp add: bit_eq_iff)
   apply (auto simp add: bit_simps)
@@ -277,7 +334,7 @@ lemma mov_subgoal6_4: "and 1 (rex >> Suc 0) = (0::u8) \<Longrightarrow>
   apply (simp add: eval_nat_numeral(2) eval_nat_numeral(3))
   done
 
-lemma mov_subgoal6_5: "bit rex (Suc (Suc 0)) \<Longrightarrow>
+lemma mov_subgoal12_5: "bit rex (Suc (Suc 0)) \<Longrightarrow>
     and (or (and 8 ((rex >> 2) << 3)) (and 7 (rop >> 3))) 8 = (0::u8) \<Longrightarrow> False"
   apply (simp add: bit_eq_iff)
   apply (auto simp add: bit_simps)
@@ -285,7 +342,7 @@ lemma mov_subgoal6_5: "bit rex (Suc (Suc 0)) \<Longrightarrow>
   apply (simp add: eval_nat_numeral(2) eval_nat_numeral(3))
   done
 
-lemma mov_subgoal6_6: "bit rex 0 \<Longrightarrow>
+lemma mov_subgoal12_6: "bit rex 0 \<Longrightarrow>
     and (or (and 8 (rex << 3)) (and 7 rop)) 8 = (0::u8) \<Longrightarrow> False"
   apply (simp add: bit_eq_iff)
   apply (auto simp add: bit_simps)
@@ -293,7 +350,7 @@ lemma mov_subgoal6_6: "bit rex 0 \<Longrightarrow>
   apply (simp add: eval_nat_numeral(2) eval_nat_numeral(3))
   done
 
-lemma mov_subgoal6: "and 15 ((rex::u8) >> 4) = 4 \<Longrightarrow>
+lemma mov_subgoal12: "and 15 ((rex::u8) >> 4) = 4 \<Longrightarrow>
     and 1 (rex >> 3) = 1 \<Longrightarrow>
     and 1 (rex >> Suc 0) = 0 \<Longrightarrow>
     n < 8 \<Longrightarrow>
@@ -433,7 +490,7 @@ lemma mov_subgoal6: "and 15 ((rex::u8) >> 4) = 4 \<Longrightarrow>
         done
       done
     done
-  done
+  done *)
 
 lemma mov_goal_0: " and 15 ((rex::u8) >> 4) = 4 \<Longrightarrow>
     and 1 (rex >> 3) = 1 \<Longrightarrow>
@@ -457,7 +514,8 @@ lemma mov_goal_0: " and 15 ((rex::u8) >> 4) = 4 \<Longrightarrow>
     subgoal using mov_subgoal3 by blast
     subgoal using mov_subgoal4 by blast
     subgoal using mov_subgoal5 by blast
-    subgoal using mov_subgoal6 [of rex n rop] by blast
+    subgoal using mov_subgoal6 by blast
+    subgoal using mov_subgoal12 [of rex n rop] by blast
     done
   done
 (* 64 = 0b1000000
