theory/x64ConsistencyProof2Pmov1.thy
@@ -9,21 +9,14 @@ lemma and_8_shl_3: "and (8::u8) (rex << 3) = 0 \<or> and (8::u8) (rex << 3) = 8"
   apply (auto simp add: bit_eq_iff bit_simps)
   subgoal for n na
     by (metis bit_numeral_Bit0_Suc_iff bot_nat_0.extremum_strict leI less_Suc_eq not_bit_numeral_Bit0_0 numeral_3_eq_3)
-  subgoal for n na
-    apply (cases n, simp_all)
-    subgoal for n1
-      apply (cases n1, simp_all)
-      subgoal for n2
-        apply (cases n2, simp_all)
-        subgoal for n3
-          apply (cases n3, simp_all)
+  subgoal for n na apply (cases n, simp_all)
+    subgoal for n1 apply (cases n1, simp_all)
+      subgoal for n2 apply (cases n2, simp_all)
+        subgoal for n3 apply (cases n3, simp_all)
           apply (cases na, simp_all)
-          subgoal for b1
-            apply (cases b1, simp_all)
-            subgoal for b2
-              apply (cases b2, simp_all)
-              subgoal for b3
-                apply (cases b3, simp_all)
+          subgoal for b1 apply (cases b1, simp_all)
+            subgoal for b2 apply (cases b2, simp_all)
+              subgoal for b3 apply (cases b3, simp_all)
                 done
               done
             done
@@ -35,18 +28,12 @@ lemma and_8_shl_3: "and (8::u8) (rex << 3) = 0 \<or> and (8::u8) (rex << 3) = 8"
 
 lemma and_64_shl_6: "(and (64::u8) (rex << 6)) = 0 \<or> (and (64::u8) (rex << 6)) = 64"
   apply (auto simp add: bit_eq_iff bit_simps)
-  subgoal for n na
-    apply (cases n, simp_all)
-    subgoal for n1
-      apply (cases n1, simp_all)
-      subgoal for n2
-        apply (cases n2, simp_all)
-        subgoal for n3
-          apply (cases n3, simp_all)
-          subgoal for n4
-            apply (cases n4, simp_all)
-            subgoal for n5
-              apply (cases n5, simp_all)
+  subgoal for n na apply (cases n, simp_all)
+    subgoal for n1 apply (cases n1, simp_all)
+      subgoal for n2 apply (cases n2, simp_all)
+        subgoal for n3 apply (cases n3, simp_all)
+          subgoal for n4 apply (cases n4, simp_all)
+            subgoal for n5 apply (cases n5, simp_all)
               done
             done
           done
@@ -54,33 +41,20 @@ lemma and_64_shl_6: "(and (64::u8) (rex << 6)) = 0 \<or> (and (64::u8) (rex << 6
       done
     done
     
-  subgoal for n na
-    apply (cases n, simp_all)
-    subgoal for n1
-      apply (cases n1, simp_all)
-      subgoal for n2
-        apply (cases n2, simp_all)
-        subgoal for n3
-          apply (cases n3, simp_all)
-          subgoal for n4
-            apply (cases n4, simp_all)
-            subgoal for n5
-              apply (cases n5, simp_all)
-              subgoal for n6
-                apply (cases n6, simp_all)
+  subgoal for n na apply (cases n, simp_all)
+    subgoal for n1 apply (cases n1, simp_all)
+      subgoal for n2 apply (cases n2, simp_all)
+        subgoal for n3 apply (cases n3, simp_all)
+          subgoal for n4 apply (cases n4, simp_all)
+            subgoal for n5 apply (cases n5, simp_all)
+              subgoal for n6 apply (cases n6, simp_all)
                 apply (cases na, simp_all)
-                subgoal for b1
-                  apply (cases b1, simp_all)
-                  subgoal for b2
-                    apply (cases b2, simp_all)
-                    subgoal for b3
-                      apply (cases b3, simp_all)
-                      subgoal for b4
-                        apply (cases b4, simp_all)
-                        subgoal for b5
-                          apply (cases b5, simp_all)
-                          subgoal for b6
-                            apply (cases b6, simp_all)
+                subgoal for b1 apply (cases b1, simp_all)
+                  subgoal for b2 apply (cases b2, simp_all)
+                    subgoal for b3 apply (cases b3, simp_all)
+                      subgoal for b4 apply (cases b4, simp_all)
+                        subgoal for b5 apply (cases b5, simp_all)
+                          subgoal for b6 apply (cases b6, simp_all)
                             done
                           done
                         done
@@ -100,24 +74,16 @@ lemma [simp]: "and 3 ((rop::u8) >> 6) = 3 \<Longrightarrow> n < 8 \<Longrightarr
   apply (simp add: bit_eq_iff)
   apply (auto simp add: bit_simps)
   apply (cases n, simp_all)
-  subgoal for n1
-    apply (cases n1, simp_all)
-    subgoal for n2
-      apply (cases n2, simp_all)
-      subgoal for n3
-        apply (cases n3, simp_all)
-        subgoal for n4
-          apply (cases n4, simp_all)
-          subgoal for n5
-            apply (cases n5, simp_all)
-            subgoal for n6
-              apply (cases n6, simp_all)
-              subgoal
-                apply (drule_tac x="0" in spec)
+  subgoal for n1 apply (cases n1, simp_all)
+    subgoal for n2 apply (cases n2, simp_all)
+      subgoal for n3 apply (cases n3, simp_all)
+        subgoal for n4 apply (cases n4, simp_all)
+          subgoal for n5 apply (cases n5, simp_all)
+            subgoal for n6 apply (cases n6, simp_all)
+              subgoal apply (drule_tac x="0" in spec)
                 apply (simp add: numeral_eq_Suc)
                 done
-              subgoal
-                apply (drule_tac x="1" in spec)
+              subgoal apply (drule_tac x="1" in spec)
                 apply (simp add: numeral_eq_Suc)
                 done
               done
@@ -133,18 +99,12 @@ lemma [simp]: "and 3 ((rop::u8) >> 6) = 3 \<Longrightarrow> n < 8 \<Longrightarr
   apply (simp add: bit_eq_iff)
   apply (auto simp add: bit_simps)
   apply (cases n, simp_all)
-  subgoal for n1
-    apply (cases n1, simp_all)
-    subgoal for n2
-      apply (cases n2, simp_all)
-      subgoal for n3
-        apply (cases n3, simp_all)
-        subgoal for n4
-          apply (cases n4, simp_all)
-          subgoal for n5
-            apply (cases n5, simp_all)
-            subgoal for n6
-              apply (cases n6, simp_all)
+  subgoal for n1 apply (cases n1, simp_all)
+    subgoal for n2 apply (cases n2, simp_all)
+      subgoal for n3 apply (cases n3, simp_all)
+        subgoal for n4 apply (cases n4, simp_all)
+          subgoal for n5 apply (cases n5, simp_all)
+            subgoal for n6 apply (cases n6, simp_all)
               done
             done
           done
@@ -158,10 +118,8 @@ lemma [simp]: "and 3 ((rop::u8) >> 6) = 3 \<Longrightarrow> n < 8 \<Longrightarr
   apply (simp add: bit_eq_iff)
   apply (auto simp add: bit_simps)
   apply (cases n, simp_all)
-  subgoal for n1
-    apply (cases n1, simp_all)
-    subgoal for n2
-      apply (cases n2, simp_all)
+  subgoal for n1 apply (cases n1, simp_all)
+    subgoal for n2 apply (cases n2, simp_all)
       done
     done
   done
@@ -172,18 +130,12 @@ lemma mov_subgoal1 [simp]: "and 3 ((rop::u8) >> 6) = 3 \<Longrightarrow>
   apply (simp add: bit_eq_iff)
   apply (auto simp add: bit_simps)
   apply (cases n, simp_all)
-  subgoal for n1
-    apply (cases n1, simp_all)
-    subgoal for n2
-      apply (cases n2, simp_all)
-      subgoal for n3
-        apply (cases n3, simp_all)
-        subgoal for n4
-          apply (cases n4, simp_all)
-          subgoal for n5
-            apply (cases n5, simp_all)
-            subgoal for n6
-              apply (cases n6, simp_all)
+  subgoal for n1 apply (cases n1, simp_all)
+    subgoal for n2 apply (cases n2, simp_all)
+      subgoal for n3 apply (cases n3, simp_all)
+        subgoal for n4 apply (cases n4, simp_all)
+          subgoal for n5 apply (cases n5, simp_all)
+            subgoal for n6 apply (cases n6, simp_all)
               done
             done
           done
@@ -198,12 +150,9 @@ lemma mov_subgoal2 [simp]: "and 3 ((rop::u8) >> 6) = 3 \<Longrightarrow>
   apply (simp add: bit_eq_iff)
   apply (auto simp add: bit_simps)
   apply (cases n, simp_all)
-  subgoal for n1
-    apply (cases n1, simp_all)
-    subgoal for n2
-      apply (cases n2, simp_all)
-      subgoal for n3
-        apply (cases n3, simp_all)
+  subgoal for n1 apply (cases n1, simp_all)
+    subgoal for n2 apply (cases n2, simp_all)
+      subgoal for n3 apply (cases n3, simp_all)
         done
       done
     done
@@ -214,34 +163,87 @@ lemma  [simp]: "and 3 ((rop::u8) >> 6) = 3 \<Longrightarrow> n < 8 \<Longrightar
   apply (simp add: bit_eq_iff)
   apply (auto simp add: bit_simps)
   apply (cases n, simp_all)
-  subgoal for n1
-    apply (cases n1, simp_all)
-    subgoal for n2
-      apply (cases n2, simp_all)
+  subgoal for n1 apply (cases n1, simp_all)
+    subgoal for n2 apply (cases n2, simp_all)
       done
     done
   done
 
 lemma mov_subgoal3 [simp]: "and 3 ((rop::u8) >> 6) = 3 \<Longrightarrow>
+    bit rop n \<Longrightarrow> \<not> bit (192::int) n \<Longrightarrow>
+    \<not> 3 \<le> n \<Longrightarrow> bit (8::int) n \<Longrightarrow> False"
+  apply (simp add: bit_eq_iff)
+  apply (auto simp add: bit_simps)
+  apply (cases n, simp_all)
+  subgoal for n1 apply (cases n1, simp_all)
+    subgoal for n2 apply (cases n2, simp_all)
+      done
+    done
+  done
+
+lemma mov_subgoal4 [simp]: "and 3 ((rop::u8) >> 6) = 3 \<Longrightarrow>
+    bit rop n \<Longrightarrow> \<not> bit (192::int) n \<Longrightarrow>
+    \<not> 3 \<le> n \<Longrightarrow> bit (56::int) n \<Longrightarrow> False"
+  apply (simp add: bit_eq_iff)
+  apply (auto simp add: bit_simps)
+  apply (cases n, simp_all)
+  subgoal for n1 apply (cases n1, simp_all)
+    subgoal for n2 apply (cases n2, simp_all)
+      done
+    done
+  done
+
+lemma mov_subgoal5 [simp]: "and 3 ((rop::u8) >> 6) = 3 \<Longrightarrow>
     n < 8 \<Longrightarrow> bit rop n \<Longrightarrow> \<not> bit (192::int) n \<Longrightarrow>
     bit (8::int) n \<Longrightarrow> bit (71::int) n \<Longrightarrow> False"
   apply (simp add: bit_eq_iff)
   apply (auto simp add: bit_simps)
   apply (cases n, simp_all)
-  subgoal for n1
-    apply (cases n1, simp_all)
-    subgoal for n2
-      apply (cases n2, simp_all)
+  subgoal for n1 apply (cases n1, simp_all)
+    subgoal for n2 apply (cases n2, simp_all)
+      subgoal for n3 apply (cases n3, simp_all)
+        done
+      done
+    done
+  done
+
+lemma [simp]: "and 3 ((rop::u8) >> 6) = 3 \<Longrightarrow>
+    n < 8 \<Longrightarrow> bit rop n \<Longrightarrow> \<not> bit (192::int) n \<Longrightarrow>
+    bit (56::int) n \<Longrightarrow> bit rop (3 + (n - 3))"
+  apply (simp add: bit_eq_iff)
+  apply (auto simp add: bit_simps)
+  apply (cases n, simp_all)
+  subgoal for n1 apply (cases n1, simp_all)
+    subgoal for n2 apply (cases n2, simp_all)
       subgoal for n3
-        apply (cases n3, simp_all)
+        by (metis Suc3_eq_add_3) 
+      done
+    done
+  done
+
+lemma mov_subgoal6 [simp]: "and 3 ((rop::u8) >> 6) = 3 \<Longrightarrow>
+    n < 8 \<Longrightarrow> bit rop n \<Longrightarrow> \<not> bit (192::int) n \<Longrightarrow>
+    bit (56::int) n \<Longrightarrow> bit (71::int) n \<Longrightarrow> False"
+  apply (simp add: bit_eq_iff)
+  apply (auto simp add: bit_simps)
+  apply (cases n, simp_all)
+  subgoal for n1 apply (cases n1, simp_all)
+    subgoal for n2 apply (cases n2, simp_all)
+      subgoal for n3 apply (cases n3, simp_all)
+        subgoal for n4 apply (cases n4, simp_all)
+          subgoal for n5 apply (cases n5, simp_all)
+            done
+          done
         done
       done
     done
   done
 
 lemma mov_subgoal1_1: "and 3 ((rop::u8) >> 6) = 3 \<Longrightarrow>
-  or (or 192 (and 56 (and (and 56 ((rop >> 3) << 3)) (- 72))))
-     (and 7 (and (and 7 rop) (- 9))) =
+    or 192
+     (and (or (and 56 (and (and 56 ((rop >> 3) << 3)) (- 72)))
+            (and (and 7 (and (and 7 rop) (- 9))) (- 57)))
+       (- 193)) =
     rop"
   apply (rule bit_eqI)
   subgoal for n
@@ -250,24 +252,22 @@ lemma mov_subgoal1_1: "and 3 ((rop::u8) >> 6) = 3 \<Longrightarrow>
     subgoal using mov_subgoal1 by blast
     subgoal using mov_subgoal2 by blast
     subgoal using mov_subgoal3 by blast
+    subgoal using mov_subgoal4 by blast
+    subgoal using mov_subgoal5 by blast
+    subgoal using mov_subgoal6 by blast
     done
   done
 
-lemma mov_subgoal4: "and 3 ((rop::u8) >> 6) = 3 \<Longrightarrow> n < 8 \<Longrightarrow>
+lemma mov_subgoal7: "and 3 ((rop::u8) >> 6) = 3 \<Longrightarrow> n < 8 \<Longrightarrow>
   bit (56::int) n \<Longrightarrow> bit (64::int) n \<Longrightarrow> bit rop n"
   apply (simp add: bit_eq_iff)
   apply (auto simp add: bit_simps)
   apply (cases n, simp_all)
-  subgoal for n1
-    apply (cases n1, simp_all)
-    subgoal for n2
-      apply (cases n2, simp_all)
-      subgoal for n3
-        apply (cases n3, simp_all)
-        subgoal for n4
-          apply (cases n4, simp_all)
-          subgoal for n5
-            apply (cases n5, simp_all)
+  subgoal for n1 apply (cases n1, simp_all)
+    subgoal for n2 apply (cases n2, simp_all)
+      subgoal for n3 apply (cases n3, simp_all)
+        subgoal for n4 apply (cases n4, simp_all)
+          subgoal for n5 apply (cases n5, simp_all)
             done
           done
         done
@@ -275,21 +275,19 @@ lemma mov_subgoal4: "and 3 ((rop::u8) >> 6) = 3 \<Longrightarrow> n < 8 \<Longri
     done
   done
 
-lemma mov_subgoal5 [simp]: "and 3 ((rop::u8) >> 6) = 3 \<Longrightarrow> n < 8 \<Longrightarrow>
+lemma mov_subgoal8 [simp]: "and 3 ((rop::u8) >> 6) = 3 \<Longrightarrow> n < 8 \<Longrightarrow>
     bit rop n \<Longrightarrow> \<not> bit (192::int) n \<Longrightarrow> \<not> bit (7::int) n \<Longrightarrow>
     \<not> bit (64::int) n \<Longrightarrow> bit (71::int) n \<Longrightarrow> False"
   apply (simp add: bit_eq_iff)
   apply (auto simp add: bit_simps)
   apply (cases n, simp_all)
-  subgoal for n1
-    apply (cases n1, simp_all)
-    subgoal for n2
-      apply (cases n2, simp_all)
+  subgoal for n1 apply (cases n1, simp_all)
+    subgoal for n2 apply (cases n2, simp_all)
       done
     done
   done
 
-lemma mov_subgoal6 [simp]: "and 3 ((rop::u8) >> 6) = 3 \<Longrightarrow> n < 8 \<Longrightarrow>
+lemma mov_subgoal9 [simp]: "and 3 ((rop::u8) >> 6) = 3 \<Longrightarrow> n < 8 \<Longrightarrow>
   bit rop n \<Longrightarrow> \<not> bit (192::int) n \<Longrightarrow> \<not> bit (56::int) n \<Longrightarrow> bit (8::int) n \<Longrightarrow> False"
   apply (simp add: bit_eq_iff)
   apply (auto simp add: bit_simps)
@@ -322,7 +320,7 @@ lemma [simp]: "and 3 ((rop::u8) >> 6) = 3 \<Longrightarrow> n < 8 \<Longrightarr
     done
   done
 
-lemma mov_subgoal7 [simp]: "and 3 ((rop::u8) >> 6) = 3 \<Longrightarrow> n < 8 \<Longrightarrow>
+lemma mov_subgoal10 [simp]: "and 3 ((rop::u8) >> 6) = 3 \<Longrightarrow> n < 8 \<Longrightarrow>
   bit rop n \<Longrightarrow> \<not> bit (192::int) n \<Longrightarrow> \<not> bit (64::int) n \<Longrightarrow>
   bit (8::int) n \<Longrightarrow> bit (71::int) n \<Longrightarrow> False"
   apply (simp add: bit_eq_iff)
@@ -344,10 +342,10 @@ lemma mov_subgoal1_2: "and 3 ((rop::u8) >> 6) = 3 \<Longrightarrow>
   subgoal for n
     apply (simp add: bit_or_iff)
     apply (auto simp add: bit_simps)
-    subgoal using mov_subgoal4 by blast
-    subgoal using mov_subgoal5 by blast
-    subgoal using mov_subgoal6 by blast
     subgoal using mov_subgoal7 by blast
+    subgoal using mov_subgoal8 by blast
+    subgoal using mov_subgoal9 by blast
+    subgoal using mov_subgoal10 by blast
     done
   done
 
@@ -364,7 +362,7 @@ lemma [simp]: "and 3 ((rop::u8) >> 6) = 3 \<Longrightarrow> n < 8 \<Longrightarr
     done
   done
 
-lemma mov_subgoal8 [simp]: "and 3 ((rop::u8) >> 6) = 3 \<Longrightarrow> n < 8 \<Longrightarrow>
+lemma mov_subgoal11 [simp]: "and 3 ((rop::u8) >> 6) = 3 \<Longrightarrow> n < 8 \<Longrightarrow>
   bit rop n \<Longrightarrow> \<not> bit (192::int) n \<Longrightarrow> \<not> bit (7::int) n \<Longrightarrow> bit (71::int) n \<Longrightarrow> False"
   apply (simp add: bit_eq_iff)
   apply (auto simp add: bit_simps)
@@ -389,7 +387,7 @@ lemma mov_subgoal8 [simp]: "and 3 ((rop::u8) >> 6) = 3 \<Longrightarrow> n < 8 \
     done
   done
 
-lemma mov_subgoal9: "and 3 ((rop::u8) >> 6) = 3 \<Longrightarrow> n < 8 \<Longrightarrow>
+lemma mov_subgoal12: "and 3 ((rop::u8) >> 6) = 3 \<Longrightarrow> n < 8 \<Longrightarrow>
   bit rop n \<Longrightarrow> \<not> bit (192::int) n \<Longrightarrow> \<not> bit (8::int) n \<Longrightarrow> \<not> bit (56::int) n \<Longrightarrow> bit (7::int) n"
   apply (simp add: bit_eq_iff)
   apply (auto simp add: bit_simps)
@@ -414,7 +412,7 @@ lemma mov_subgoal9: "and 3 ((rop::u8) >> 6) = 3 \<Longrightarrow> n < 8 \<Longri
     done
   done
 
-lemma mov_subgoal10 [simp]: "and 3 ((rop::u8) >> 6) = 3 \<Longrightarrow> n < 8 \<Longrightarrow>
+lemma mov_subgoal13 [simp]: "and 3 ((rop::u8) >> 6) = 3 \<Longrightarrow> n < 8 \<Longrightarrow>
   bit rop n \<Longrightarrow> \<not> bit (192::int) n \<Longrightarrow> \<not> bit (8::int) n \<Longrightarrow>
   \<not> bit (7::int) n \<Longrightarrow> bit (71::int) n \<Longrightarrow> False"
   apply (simp add: bit_eq_iff)
@@ -448,13 +446,13 @@ lemma mov_subgoal1_3: "and 3 ((rop::u8) >> 6) = 3 \<Longrightarrow>
   subgoal for n
     apply (simp add: bit_or_iff)
     apply (auto simp add: bit_simps)
-    subgoal using mov_subgoal8 by blast
-    subgoal using mov_subgoal9 by blast
-    subgoal using mov_subgoal10 by blast
+    subgoal using mov_subgoal11 by blast
+    subgoal using mov_subgoal12 by blast
+    subgoal using mov_subgoal13 by blast
     done
   done
 
-lemma mov_subgoal11: "and 3 ((rop::u8) >> 6) = 3 \<Longrightarrow> n < 8 \<Longrightarrow>
+lemma mov_subgoal14: "and 3 ((rop::u8) >> 6) = 3 \<Longrightarrow> n < 8 \<Longrightarrow>
   bit (56::int) n \<Longrightarrow> bit (64::int) n \<Longrightarrow> bit rop n"
   apply (simp add: bit_eq_iff)
   apply (auto simp add: bit_simps)
@@ -476,7 +474,7 @@ lemma mov_subgoal11: "and 3 ((rop::u8) >> 6) = 3 \<Longrightarrow> n < 8 \<Longr
     done
   done
 
-lemma mov_subgoal12 [simp]: "and 3 ((rop::u8) >> 6) = 3 \<Longrightarrow> n < 8 \<Longrightarrow>
+lemma mov_subgoal15 [simp]: "and 3 ((rop::u8) >> 6) = 3 \<Longrightarrow> n < 8 \<Longrightarrow>
   bit rop n \<Longrightarrow> \<not> bit (192::int) n \<Longrightarrow> \<not> bit (7::int) n \<Longrightarrow>
   \<not> bit (64::int) n \<Longrightarrow> bit (71::int) n \<Longrightarrow> False"
   apply (simp add: bit_eq_iff)
@@ -490,7 +488,7 @@ lemma mov_subgoal12 [simp]: "and 3 ((rop::u8) >> 6) = 3 \<Longrightarrow> n < 8 
     done
   done
 
-lemma mov_subgoal13 : "and 3 ((rop::u8) >> 6) = 3 \<Longrightarrow> n < 8 \<Longrightarrow>
+lemma mov_subgoal16 : "and 3 ((rop::u8) >> 6) = 3 \<Longrightarrow> n < 8 \<Longrightarrow>
   bit rop n \<Longrightarrow> \<not> bit (192::int) n \<Longrightarrow> \<not> bit (8::int) n \<Longrightarrow>
   \<not> bit (56::int) n \<Longrightarrow> bit (7::int) n"
   apply (simp add: bit_eq_iff)
@@ -516,7 +514,7 @@ lemma mov_subgoal13 : "and 3 ((rop::u8) >> 6) = 3 \<Longrightarrow> n < 8 \<Long
     done
   done
 
-lemma mov_subgoal14 : "and 3 ((rop::u8) >> 6) = 3 \<Longrightarrow> n < 8 \<Longrightarrow>
+lemma mov_subgoal17 : "and 3 ((rop::u8) >> 6) = 3 \<Longrightarrow> n < 8 \<Longrightarrow>
   bit rop n \<Longrightarrow> \<not> bit (192::int) n \<Longrightarrow> \<not> bit (8::int) n \<Longrightarrow>
   \<not> bit (64::int) n \<Longrightarrow> \<not> bit (7::int) n \<Longrightarrow> bit (71::int) n \<Longrightarrow> False"
   apply (simp add: bit_eq_iff)
@@ -538,10 +536,10 @@ lemma mov_subgoal1_4: "and 3 ((rop::u8) >> 6) = 3 \<Longrightarrow>
   subgoal for n
     apply (simp add: bit_or_iff)
     apply (auto simp add: bit_simps)
-    subgoal using mov_subgoal11 by blast
-    subgoal using mov_subgoal12 by blast
-    subgoal using mov_subgoal13 by blast
     subgoal using mov_subgoal14 by blast
+    subgoal using mov_subgoal15 by blast
+    subgoal using mov_subgoal16 by blast
+    subgoal using mov_subgoal17 by blast
     done
   done
 
@@ -550,9 +548,7 @@ lemma mov_goal_1: "and 3 ((rop::u8) >> 6) = 3 \<Longrightarrow>
      (bitfield_insert_u8 3 (Suc 0) (and 7 (rop >> 3)) (and 1 (rex >> 2)))
      (bitfield_insert_u8 3 (Suc 0) (and 7 rop) (and 1 rex)) =
     rop"
-  apply (unfold construct_rex_to_u8_def construct_modsib_to_u8_def)
-  apply simp
-  apply (unfold bitfield_insert_u8_def u8_of_bool_def)
+  apply (unfold construct_rex_to_u8_def construct_modsib_to_u8_def bitfield_insert_u8_def)
   apply simp
   apply (insert and_8_shl_3 [of rex])
   apply (erule disjE, simp_all)
@@ -560,13 +556,13 @@ lemma mov_goal_1: "and 3 ((rop::u8) >> 6) = 3 \<Longrightarrow>
     apply (insert and_64_shl_6 [of "rex >> 2"])
     apply (erule disjE, simp_all)
     subgoal using mov_subgoal1_1 by blast
-    subgoal using mov_subgoal1_2 by blast
+    subgoal sorry (* using mov_subgoal1_2 by blast *) (**r change the proof goal of mov_subgoal1_2 *)
     done
   subgoal
     apply (insert and_64_shl_6 [of "rex >> 2"])
     apply (erule disjE, simp_all)
-    subgoal using mov_subgoal1_3 by blast
-    subgoal using mov_subgoal1_4 by blast
+    subgoal using mov_subgoal1_3 by blast (**r same *)
+    subgoal using mov_subgoal1_4 by blast (**r same *)
     done
   done
 
